Get le_bytes_to_seq_quad32_to_bytes lemma to go through by removing the unfold on seq_map

src/arch/Types_i.fst
@@ -66,3 +66,83 @@ let push_pop_xmm (x y:quad32) : Lemma
    =
 //   assert (nat_to_two 32 (hi64 x) == two_select (four_to_two_two x) 1);
    ()
+
+
+#reset-options "--z3rlimit 10 --max_fuel 0 --max_ifuel 0 --using_facts_from '* -FStar.Seq.Properties'"
+let le_bytes_to_seq_quad32_to_bytes (b:quad32) :
+  Lemma (le_bytes_to_seq_quad32 (le_quad32_to_bytes b) == create 1 b)
+(* This expands into showing:
+   le_bytes_to_seq_quad32 (le_quad32_to_bytes b)
+ == { definition of le_bytes_to_seq_quad32 }
+   seq_to_seq_four_LE (seq_nat8_to_seq_nat32_LE (le_quad32_to_bytes b))
+ == { definition of le_quad32_to_bytes }
+   seq_to_seq_four_LE (seq_nat8_to_seq_nat32_LE (seq_four_to_seq_LE (seq_map (nat_to_four 8) (four_to_seq_LE b))))
+ == { definition of seq_nat8_to_seq_nat32_LE }
+   seq_to_seq_four_LE (seq_map (four_to_nat 8) (seq_to_seq_four_LE (seq_four_to_seq_LE (seq_map (nat_to_four 8) (four_to_seq_LE b)))))
+ == { seq_to_seq_four_to_seq_LE (seq_map (nat_to_four 8) (four_to_seq_LE b)) }
+   seq_to_seq_four_LE (seq_map (four_to_nat 8) (seq_map (nat_to_four 8) (four_to_seq_LE b)))
+ == { seq_map_inverses (four_to_nat 8) (nat_to_four 8) (four_to_seq_LE b) }
+   seq_to_seq_four_LE (four_to_seq_LE b)
+ == { four_to_seq_LE_is_seq_four_to_seq_LE b }
+   seq_to_seq_four_LE (seq_four_to_seq_LE (create 1 b))
+ == { seq_to_seq_four_to_seq_LE (create 1 b) }
+   create 1 b
+ *)
+  =
+  seq_to_seq_four_to_seq_LE (seq_map (nat_to_four 8) (four_to_seq_LE b));
+  seq_map_inverses (nat_to_four 8) (four_to_nat 8) (four_to_seq_LE b);
+  four_to_seq_LE_is_seq_four_to_seq_LE b;
+  seq_to_seq_four_to_seq_LE (create 1 b) ;
+  (*
+  assert (le_bytes_to_seq_quad32 (le_quad32_to_bytes b) == seq_to_seq_four_LE (seq_nat8_to_seq_nat32_LE (le_quad32_to_bytes b)));
+  assert (le_quad32_to_bytes b == seq_four_to_seq_LE (seq_map (nat_to_four 8) (four_to_seq_LE b)));
+  assert ((le_bytes_to_seq_quad32 (le_quad32_to_bytes b)) == 
+          (seq_to_seq_four_LE (seq_nat8_to_seq_nat32_LE (seq_four_to_seq_LE (seq_map (nat_to_four 8) (four_to_seq_LE b)))))
+          ); 
+  let annoying_definition_expander (x:seq nat8{length x % 4 == 0}) :
+    Lemma ( (seq_nat8_to_seq_nat32_LE (x)) ==
+           (seq_map (four_to_nat 8) (seq_to_seq_four_LE x) )) = () in
+
+  let (s:seq nat8{length s % 4 == 0}) = seq_four_to_seq_LE (seq_map (nat_to_four 8) (four_to_seq_LE b)) in
+  //annoying_definition_expander s;
+  assert ( (seq_nat8_to_seq_nat32_LE (s)) ==
+           (seq_map (four_to_nat 8) (seq_to_seq_four_LE s) ));
+           
+  assert ( (le_bytes_to_seq_quad32 (le_quad32_to_bytes b)) ==
+           seq_to_seq_four_LE (seq_map (four_to_nat 8) (seq_to_seq_four_LE s)) );           
+  assert (seq_to_seq_four_LE (seq_four_to_seq_LE (seq_map (nat_to_four 8) (four_to_seq_LE b))) ==
+          seq_map (nat_to_four 8) (four_to_seq_LE b));
+  assert ( (le_bytes_to_seq_quad32 (le_quad32_to_bytes b)) ==
+           seq_to_seq_four_LE (seq_map (four_to_nat 8) (seq_map (nat_to_four 8) (four_to_seq_LE b))) );
+  (*
+  assert ( (seq_to_seq_four_LE (seq_map (four_to_nat 8) (seq_to_seq_four_LE (seq_four_to_seq_LE (seq_map (nat_to_four 8) (four_to_seq_LE b))))))
+                   ==
+                  (seq_to_seq_four_LE (seq_map (four_to_nat 8) (seq_map (nat_to_four 8) (four_to_seq_LE b)))));
+                  *)
+  //assert (equal (le_bytes_to_seq_quad32 (le_quad32_to_bytes b)) (create 1 b));
+  //admit();
+  *)
+  ()
+ 
+
+(*
+  Let s4 = seq_map (nat_to_four 8) (four_to_seq_LE b) in
+  let s4wrapped = seq_to_seq_four_LE (seq_four_to_seq_LE s4) in
+  assert (s4wrapped == s4);
+  seq_map_inverses (nat_to_four 8) (four_to_nat 8) (four_to_seq_LE b);
+  seq_to_seq_four_to_seq_LE (create 1 b);
+  four_to_seq_LE_is_seq_four_to_seq_LE b;
+
+  assert (le_bytes_to_seq_quad32 (le_quad32_to_bytes b) ==
+            seq_to_seq_four_LE (seq_nat8_to_seq_nat32_LE (le_quad32_to_bytes b)));
+  assert (equal (le_quad32_to_bytes b) (seq_four_to_seq_LE (seq_map (nat_to_four 8) (four_to_seq_LE b))));
+  (*
+  assert (equal (seq_nat8_to_seq_nat32_LE (le_quad32_to_bytes b)) 
+                (seq_nat8_to_seq_nat32_LE (seq_four_to_seq_LE (seq_map (nat_to_four 8) (four_to_seq_LE b)))));
+  *)
+  admit();
+  assert (equal (seq_to_seq_four_LE (seq_nat8_to_seq_nat32_LE (le_quad32_to_bytes b)))
+          (seq_to_seq_four_LE (seq_nat8_to_seq_nat32_LE (seq_four_to_seq_LE (seq_map (nat_to_four 8) (four_to_seq_LE b))))));
+  admit();
+  ()
+*)
